pulse/share/steel/examples/pulse/dice/cbor/CBOR.Spec.fsti
@@ -24,3 +24,61 @@ val serialize_cbor_nonempty
 (* 4.2.1 Deterministically encoded CBOR: The keys in every map MUST be sorted in the bytewise lexicographic order of their deterministic encodings. *)
 
 val deterministically_encoded_cbor_map_key_order : Ghost.erased (raw_data_item -> raw_data_item -> bool)
+
+val deterministically_encoded_cbor_map_key_order_irrefl
+  (x: raw_data_item)
+: Lemma
+  (Ghost.reveal deterministically_encoded_cbor_map_key_order x x == false)
+  [SMTPat (Ghost.reveal deterministically_encoded_cbor_map_key_order x x)]
+
+val deterministically_encoded_cbor_map_key_order_trans
+  (x y z: raw_data_item)
+: Lemma
+  (requires (Ghost.reveal deterministically_encoded_cbor_map_key_order x y == true /\ Ghost.reveal deterministically_encoded_cbor_map_key_order y z == true))
+  (ensures (Ghost.reveal deterministically_encoded_cbor_map_key_order x z == true))
+  [SMTPat (Ghost.reveal deterministically_encoded_cbor_map_key_order x y); SMTPat (Ghost.reveal deterministically_encoded_cbor_map_key_order y z)]
+
+let rec list_ghost_assoc
+  (#key: Type)
+  (#value: Type)
+  (k: key)
+  (m: list (key & value))
+: GTot (option value)
+  (decreases m)
+= match m with
+  | [] -> None
+  | (k', v') :: m' ->
+    if FStar.StrongExcludedMiddle.strong_excluded_middle (k == k')
+    then Some v'
+    else list_ghost_assoc k m'
+
+val deterministically_encoded_cbor_map_key_order_assoc_ext :
+  (m1: list (raw_data_item & raw_data_item)) ->
+  (m2: list (raw_data_item & raw_data_item)) ->
+  (ext: (
+    (k: raw_data_item) ->
+    Lemma
+    (list_ghost_assoc k m1 == list_ghost_assoc k m2)
+  )) ->
+  Lemma
+  (requires (List.Tot.sorted (map_entry_order deterministically_encoded_cbor_map_key_order _) m1 /\ List.Tot.sorted (map_entry_order deterministically_encoded_cbor_map_key_order _) m2))
+  (ensures (m1 == m2))
+
+module U64 = FStar.UInt64
+
+val deterministically_encoded_cbor_map_key_order_major_type_intro
+  (v1 v2: raw_data_item)
+: Lemma
+  (requires (
+    U8.v (get_major_type v1) < U8.v (get_major_type v2)
+  ))
+  (ensures (
+    Ghost.reveal deterministically_encoded_cbor_map_key_order v1 v2 == true
+  ))
+
+val deterministically_encoded_cbor_map_key_order_int64
+  (ty: major_type_uint64_or_neg_int64)
+  (v1 v2: U64.t)
+: Lemma
+  (Ghost.reveal deterministically_encoded_cbor_map_key_order (Int64 ty v1) (Int64 ty v2) == U64.lt v1 v2)
+  [SMTPat (Ghost.reveal deterministically_encoded_cbor_map_key_order (Int64 ty v1) (Int64 ty v2))]
